rocq-brick-libstdcpp/test/mutex/custom_mutex_hpp_proof.v
@@ -1,6 +1,5 @@
 (** Provisional *)
 
-Require Import iris.algebra.lib.excl_auth.
 Require Import iris.algebra.gset.
 
 Require Import skylabs.auto.cpp.proof.
@@ -13,11 +12,143 @@ Require Import skylabs.brick.libstdcpp.cassert.spec.
 Import linearity.
 Require Import skylabs.brick.libstdcpp.test.mutex.custom_mutex_hpp.
 
-Module custom_mutex.
+(** The ghost implementation and its physical client predicates are specific
+    to [MyMutex]. The entire mutex-set pool still uses one shared ghost name. *)
+Module CustomMutexState (Sets0 : MUTEX_SETS) (Tokens0 : MUTEX_TOKENS)
+    (Owners0 : OWNER_TID) <: MUTEX_STATE.
+  Record mutex_gname : Set := MkGname {
+    pool_gname : iprop.gname;
+    invariant_gname : iprop.gname;
+    token_gname : iprop.gname;
+    owner_gname : iprop.gname;
+  }.
+  Definition gname : Set := mutex_gname * cQp.t.
+  Definition Q : Type := cQp.t.
+  Definition pool_name (γ : gname) : iprop.gname := γ.1.(pool_gname).
+  Definition inv_name (γ : gname) : iprop.gname := γ.1.(invariant_gname).
 
-  Module Spec := mutex_spec LockState.
+  Class stateG `{Σ : cpp_logic} := {
+    #[global] sets_G :: Sets0.G Σ;
+    #[global] tokens_G :: Tokens0.G Σ;
+    #[global] owners_G :: Owners0.G Σ;
+  }.
+  Definition G := @stateG.
+  Existing Class G.
+  #[global] Arguments G {_ _} Σ : assert.
+  #[global] Instance state_G `{Σ : cpp_logic} (H : G Σ) : @stateG _ _ Σ := H.
 
-  Abbreviation N := "MyMutex"%cpp_name.
+  Definition token `{Σ : cpp_logic, !G Σ}
+      (γ : gname) (q : Qp) : mpred :=
+    Tokens0.token γ.1.(token_gname) q.
+
+  Definition lock_permit `{Σ : cpp_logic, !G Σ}
+      (γ : mutex_gname) (th : thread_idT) (q : Qp) : mpred :=
+    Sets0.mutex_set_frag γ.(pool_gname) th (GSet {[γ.(invariant_gname)]}) **
+    Tokens0.token γ.(token_gname) q.
+
+  Definition owner_token `{Σ : cpp_logic, !G Σ}
+      (γ : mutex_gname) (th : thread_idT) (q : Qp) : mpred :=
+    Tokens0.given_token γ.(token_gname) q **
+    Owners0.owner_tid_frag γ.(owner_gname) (Some th).
+
+  #[global] Instance token_fractional
+      `{Σ : cpp_logic, !G Σ} γ : Fractional (token γ).
+  Proof. rewrite /token. apply Tokens0.token_fractional. Qed.
+
+  #[global] Instance token_timeless
+      `{Σ : cpp_logic, !G Σ} γ q : Timeless (token γ q).
+  Proof. rewrite /token. apply _. Qed.
+
+  #[global] Instance owner_token_timeless
+      `{Σ : cpp_logic, !G Σ} γ th q : Timeless (owner_token γ th q).
+  Proof. rewrite /owner_token. apply _. Qed.
+
+  #[global] Instance owner_token_exclusive
+      `{Σ : cpp_logic, !G Σ} γ q : Exclusive1 (fun th => owner_token γ th q).
+  Proof.
+    intros th1 th2. rewrite /owner_token.
+    apply _.
+  Qed.
+
+  (** While held, the invariant owns this thread's singleton mutex fragment
+      and the token balance. The thread retains its mutex-set authority.
+      When free, both halves of the previous owner remain in the invariant. *)
+  Definition state `{Σ : cpp_logic, !G Σ}
+      (γ : mutex_gname) (b : bool) : mpred :=
+    (if b then
+      ∃ th, Owners0.owner_tid_auth γ.(owner_gname) (Some th) **
+        Sets0.mutex_set_frag γ.(pool_gname) th (GSet {[γ.(invariant_gname)]}) **
+        Tokens0.token_not_full γ.(token_gname)
+    else
+      ∃ owner, Owners0.owner_tid_auth γ.(owner_gname) owner **
+        Owners0.owner_tid_frag γ.(owner_gname) owner **
+        Tokens0.token_full γ.(token_gname))%I.
+
+  #[global] Instance state_WeaklyObjective
+      `{Σ : cpp_logic, !G Σ} γ b :
+    WeaklyObjective (state γ b).
+  Proof. rewrite /state. destruct b; apply _. Qed.
+
+  Section state_laws.
+    Context `{Σ : cpp_logic, !G Σ}.
+
+    Lemma alloc (γpool : iprop.gname) inv_gname :
+      ⊢ |==> ∃ γ, [| γ.(pool_gname) = γpool |] ** [| γ.(invariant_gname) = inv_gname |] **
+        token (γ, (1$m)%cQp) 1 ** state γ false.
+    Proof.
+      iMod Tokens0.alloc as (gt) "[T GT]".
+      iMod (Owners0.alloc None) as (go) "[OA OF]".
+      iModIntro. iExists (MkGname γpool inv_gname gt go).
+      iSplit; first done. iSplit; first done.
+      rewrite /token /state /=. iFrame "T". iExists None.
+      iFrame "OA OF".
+      iApply Tokens0.token_full_init. iExact "GT".
+    Qed.
+
+    Lemma do_lock γ th q :
+      state γ false ** lock_permit γ th q |--
+        (|==> state γ true ** owner_token γ th q).
+    Proof.
+      rewrite /state /lock_permit /owner_token.
+      iIntros "[State [Sets T]]".
+      iDestruct "State" as (owner) "(OA & OF & Balance)".
+      iDestruct (Tokens0.acquire with "[$Balance $T]") as "[GT Balance]".
+      iMod (Owners0.owner_update γ.(owner_gname) _ _ (Some th)
+        with "[$OA $OF]") as "[OA OF]".
+      iModIntro. iFrame "GT OF". iExists th. iFrame.
+    Qed.
+
+    Lemma do_unlock γ th q :
+      state γ true ** owner_token γ th q |--
+        (|==> state γ false ** lock_permit γ th q).
+    Proof.
+      rewrite /state /owner_token /lock_permit.
+      iIntros "[State [GT OF]]".
+      iDestruct "State" as (owner) "(OA & Sets & Balance)".
+      iDestruct (observe_2 [| Some owner = Some th |] with "OA OF") as %Heq.
+      injection Heq as ->.
+      iDestruct (Tokens0.release with "[$Balance $GT]") as "[T Balance]".
+      iModIntro. iFrame "Sets T". iExists (Some th). iFrame.
+    Qed.
+
+    Lemma unlocked_owner_token γ th q :
+      state γ false ** owner_token γ th q |-- False.
+    Proof.
+      rewrite /state /owner_token. iIntros "[State [_ OF]]".
+      iDestruct "State" as (owner) "(_ & OF0 & _)".
+      iDestruct (Owners0.owner_tid_frag_exclusive with "OF0 OF") as %[].
+    Qed.
+
+    Lemma locked_full_token γ :
+      state γ true ** token (γ, (1$m)%cQp) 1 |-- False.
+    Proof.
+      rewrite /state /token. iIntros "[State T]".
+      iDestruct "State" as (th) "(_ & _ & Balance)".
+      iApply (Tokens0.token_not_full_full_token with "[$Balance $T]").
+    Qed.
+  End state_laws.
+
+  #[global] Hint Opaque token lock_permit owner_token state : sl_opacity typeclass_instances.
 
   Parameter thread_idR : ∀ `{Σ : cpp_logic, σ : genv}, cQp.t ->
     (* None if value is thread::id(), Some otherwise *)
@@ -28,6 +159,47 @@ Module custom_mutex.
       (o : option thread_idT) (p : ptr),
       WeaklyObjective (thread_idR q o p).
   #[global] Existing Instance thread_idR_WeaklyObjective.
+
+  Definition globals `{Σ : cpp_logic} {σ : genv} (q : cQp.t) : mpred :=
+    _global "std::memory_order_seq_cst" |->
+      primR "enum std::memory_order" q
+        (memory_order.to_val memory_order.seq_cst).
+
+  Definition not_locked `{Σ : cpp_logic, !G Σ} {σ : genv}
+      (this : ptr) (γ : gname) (th : thread_idT) (q : Q) : mpred :=
+    lock_permit γ.1 th γ.2 ** globals q.
+  #[global] Arguments not_locked /.
+  #[global] Arguments globals /.
+
+  (** Public ownership includes the physical owner written by [lock]. *)
+  Definition locked `{Σ : cpp_logic, !G Σ} {σ : genv}
+      (this : ptr) (γ : gname) (th : thread_idT) (q : Q) : mpred :=
+    globals q **
+      (this ,, _field "MyMutex::m_owner" |-> thread_idR 1$m (Some th) **
+        owner_token γ.1 th γ.2).
+  #[global] Arguments locked /.
+  #[global] Instance locked_timeless `{Σ : cpp_logic, !G Σ} {σ : genv}
+      this γ th q : Timeless (locked this γ th q).
+  Proof. rewrite /locked /globals. apply _. Qed.
+  #[global] Instance locked_exclusive `{Σ : cpp_logic, !G Σ} {σ : genv}
+      this γ q : Exclusive1 (fun th => locked this γ th q).
+  Proof.
+    intros th1 th2. rewrite /locked.
+    apply observe_2_sep_r. apply observe_2_sep_r. apply _.
+  Qed.
+
+End CustomMutexState.
+
+Module LockState := CustomMutexState MutexSets MutexTokens OwnerTid.
+
+(** Verify the implementation using its ghost resources and public state predicates. *)
+Module custom_mutex.
+  Module State := LockState.
+  Module Spec := mutex_spec State.
+
+  Abbreviation N := "MyMutex"%cpp_name.
+  Abbreviation thread_idR := LockState.thread_idR.
+  #[local] Hint Opaque LockState.thread_idR : sl_opacity typeclass_instances.
 
   #[local] Instance at_WeaklyObjective `{Σ : cpp_logic}
       (p : ptr) (R : Rep) `{!WeaklyObjective (R p)} :
@@ -87,52 +259,31 @@ Module custom_mutex.
       \post emp).
   End unproved_specs.
 
-  Record gname : Set := MkGname
-  { lock_state_gname : LockState.gname
-  ; cinv_gname : iprop.gname
-  }.
+  Definition gname : Set := State.mutex_gname.
+  Definition lock_state_gname (γ : gname) : State.gname := (γ, (1$m)%cQp).
+  Definition cinv_gname : gname -> iprop.gname := State.invariant_gname.
 
   Definition lock_namespace : namespace := nroot .@@ "MyMutex".
 
-  sl.lock
-  Definition lockedR `{Σ : cpp_logic} `{!LockState.G Σ} `{σ : genv}
-      (γ: gname) (thr : thread_idT) (q : cQp.t) : Rep :=
-    _field "MyMutex::m_owner" |-> thread_idR 1$m (Some thr) ** pureR (LockState.locked γ.(lock_state_gname) (Some thr) q%Qp).
-  #[global] Hint Opaque lockedR : sl_opacity typeclass_instances.
-  #[only(timeless, exclusive)] derive lockedR.
-
   Section with_Σ.
     Context `{Σ : cpp_logic, σ : genv, HAS_THREADS : !HasStdThreads Σ,
-      !LockState.G Σ}.
+      !State.G Σ}.
 
-    (** The invariant holds the thread's mutex set while the spinlock is held.
-        Its token balance supports both full and partial ownership transfers. *)
+    (** The physical lock bit agrees with the abstract ghost state. The
+        protected resources and cleared owner field are available while free. *)
     Definition mutex_inv (this : ptr) (γ : gname) (P : mpred) : mpred :=
       ∃ b : bool,
       this ,, _field "MyMutex::m_lock" |->
         atomic.R "int" 1$m (if b then 1 else 0)%Z **
-      ∃ o_owner : option thread_idT,
-      LockState.owner_tid_auth γ.(lock_state_gname) o_owner **
-      (if b then
-        ∃ th,
-          MutexSets.my_mutexes
-            γ.(lock_state_gname).(LockState.pool_namespace)
-            γ.(lock_state_gname).(LockState.pool_gname) th {[γ.(cinv_gname)]} **
-          [| o_owner = Some th |] **
-          MutexTokens.token_not_full γ.(lock_state_gname).(LockState.token_gname)
-      else
-        P **
-        (** The physical owner is cleared before [do_unlock]; the ghost owner
-            records the last acquiring thread until the next acquisition. *)
-        this ,, _field "MyMutex::m_owner" |-> thread_idR 1$m None **
-        LockState.owner_tid_frag γ.(lock_state_gname) o_owner **
-        MutexTokens.token_full γ.(lock_state_gname).(LockState.token_gname)).
+      State.state γ b **
+      if b then emp else
+        P ** this ,, _field "MyMutex::m_owner" |-> thread_idR 1$m None.
 
     Definition IR (γ : gname) (q : cQp.t) (P : mpred) : Rep :=
       structR N q$m **
       as_Rep (fun this =>
-        cinv lock_namespace γ.(cinv_gname) (mutex_inv this γ P) **
-        cinv_own γ.(cinv_gname) q
+        cinv lock_namespace (cinv_gname γ) (mutex_inv this γ P) **
+        cinv_own (cinv_gname γ) q
       ).
     Hint Opaque IR : sl_opacity typeclass_instances.
     #[only(type_ptr,cfractional,ascfractional,cfracvalid)] derive IR.
@@ -144,7 +295,7 @@ Module custom_mutex.
         primR "enum std::memory_order" q
           (memory_order.to_val memory_order.seq_cst)).
 
-    Abbreviation token := (fun g q => LockState.token g.(lock_state_gname) q).
+    Abbreviation token := (fun g q => State.token (g, (1$m)%cQp) q).
 
     cpp.spec "MyMutex::MyMutex()" as ctor_spec with
       (\exact Reduce (Spec.ctor_spec IR lock_state_gname)).
@@ -157,36 +308,28 @@ Module custom_mutex.
     Definition T : Type := gname * cQp.t * mpred.
     Abbreviation mutexR := (fun (gq : gname * cQp.t) (_ : cQp.t) P =>
       IR gq.1 gq.2 P).
-    (* the raw assertions are used for the internal do_lock() and do_unlock() *)
-    Abbreviation not_locked_raw :=
-      (fun (_ : ptr) (gq : gname * cQp.t) thr (_ : unit) =>
-        LockState.not_locked gq.1.(lock_state_gname) thr gq.2 gq.1.(cinv_gname)).
-    Abbreviation locked_raw :=
-      (fun (this : ptr) (gq : gname * cQp.t) thr (_ : unit) =>
-        (this |-> lockedR gq.1 thr gq.2)%I).
+    cpp.spec "MyMutex::do_lock()" as do_lock_spec with (
+      \this this
+      \prepost{g q P} this |-> IR g q P
+      \persist{thr} current_thread thr
+      \pre{qg} State.lock_permit g thr q ** GLOBALS qg
+      \post P ** GLOBALS qg **
+        this ,, _field "MyMutex::m_owner" |-> thread_idR 1$m None **
+        State.owner_token g thr q).
 
-    (** Locking additionally preserves the globals used by the spin loop. *)
-    Abbreviation not_locked := (fun this gq thr q' =>
-      (not_locked_raw this gq thr tt ** GLOBALS q')%I).
-    Abbreviation locked := (fun this gq thr q' =>
-      (GLOBALS q' ** locked_raw this gq thr tt)%I).
+    cpp.spec "MyMutex::do_unlock()" as do_unlock_spec with (
+      \this this
+      \prepost{g q P} this |-> IR g q P
+      \persist{thr} current_thread thr
+      \pre{qg} GLOBALS qg **
+        this ,, _field "MyMutex::m_owner" |-> thread_idR 1$m None **
+        State.owner_token g thr q
+      \pre ▷P
+      \post State.lock_permit g thr q ** GLOBALS qg).
 
-    Abbreviation raw_locked_raw :=
-      (fun (this : ptr) (gq : gname * cQp.t) thr (_ : unit) =>
-        (this ,, _field "MyMutex::m_owner" |-> thread_idR 1$m None **
-         LockState.locked gq.1.(lock_state_gname) (Some thr) gq.2)%I).
-    Abbreviation raw_locked := (fun this gq thr q' =>
-      (GLOBALS q' ** raw_locked_raw this gq thr tt)%I).
-
-    cpp.spec "MyMutex::do_lock()" as do_lock_spec with
-      (\exact Reduce (Spec.lock_spec_alt mutexR not_locked raw_locked)).
-
-    cpp.spec "MyMutex::do_unlock()" as do_unlock_spec with
-      (\exact Reduce (Spec.unlock_spec_alt mutexR not_locked_raw raw_locked_raw)).
-
-    Definition do_lock := Spec.do_lock not_locked locked.
+    Definition do_lock := Spec.do_lock (fun g => g).
     #[global] Arguments do_lock /.
-    Definition do_unlock := Spec.do_unlock not_locked_raw locked_raw.
+    Definition do_unlock := Spec.do_unlock (fun g => g).
     #[global] Arguments do_unlock /.
 
     #[global] Instance custom_mutex_basic_lockable :
@@ -196,10 +339,10 @@ Module custom_mutex.
       ; do_unlock := do_unlock }.
 
     cpp.spec "MyMutex::lock()" as lock_spec_alt with
-      (\exact Reduce (Spec.lock_spec_alt mutexR not_locked locked)).
+      (\exact Reduce (Spec.lock_spec_alt mutexR (fun g => g))).
 
     cpp.spec "MyMutex::unlock()" as unlock_spec_alt with
-      (\exact Reduce (Spec.unlock_spec_alt mutexR not_locked_raw locked_raw)).
+      (\exact Reduce (Spec.unlock_spec_alt mutexR (fun g => g))).
 
     cpp.spec "MyMutex::lock()" as lock_spec with
       (\exact Reduce
@@ -223,13 +366,13 @@ Module custom_mutex.
       \using denoteModule source
       \using{thr} current_thread thr
       \consuming{g q P} p |-> IR g q P
-      \consuming LockState.not_locked g.(lock_state_gname) thr q g.(cinv_gname)
+      \consuming State.lock_permit g thr q
       \proving{K (_ : IsExistential K)}
       std.atomic.do_exchange "int" (BASE (p,, o_field σ "MyMutex::m_lock") ) 1%Z K
       \instantiate K := (fun res => p |-> IR g q P ** [| res = 0 \/ res = 1 |]%Z **
-                          if bool_decide (res = 0) then P ** LockState.locked g.(lock_state_gname) (Some thr) q **
+                          if bool_decide (res = 0) then P ** State.owner_token g thr q **
                             p ,, _field "MyMutex::m_owner" |-> thread_idR 1$m None
-                          else LockState.not_locked g.(lock_state_gname) thr q g.(cinv_gname))
+                          else State.lock_permit g thr q)
                           \end@{mpredI}.
     Next Obligation.
       intros. iIntros "[#M Hpre]" (?? ->).
@@ -242,39 +385,33 @@ Module custom_mutex.
       iInv lock_namespace as "Inv" "Hclose".
       iDestruct "Inv" as "[Inv CO]".
       iEval (rewrite /mutex_inv) in "Inv".
-      iDestruct "Inv" as (b) "[>L Inv]".
-      iDestruct "Inv" as (oo) "[>OA State]".
+      iDestruct "Inv" as (b) "(>L & State & Resources)".
       iDestruct (fupd_mask_subseteq) as ">Y"; [ | iModIntro ]; first set_solver.
       iExists (if b then 1 else 0)%Z.
       iSplitL "L".
       { ework $usenamed=true with br_erefl. }
       iSplit.
       - iIntros "L". iMod "Y" as "_".
-        iMod ("Hclose" with "[L OA State]") as "_".
+        iMod ("Hclose" with "[L State Resources]") as "_".
         { iNext. rewrite /mutex_inv. iExists b.
           iSplitL "L"; first by ework $usenamed=true with br_erefl.
-          iExists oo. iFrame. }
+          iFrame. }
         iModIntro. iFrame.
       - iNext. iIntros "L". iMod "Y" as "_".
         destruct b.
-        + iMod ("Hclose" with "[L OA State]") as "_".
+        + iMod ("Hclose" with "[L State Resources]") as "_".
           { iNext. rewrite /mutex_inv. iExists true.
             iSplitL "L"; first by ework $usenamed=true with br_erefl.
-            iExists oo. iFrame. }
+            iFrame. }
           iModIntro. rewrite /IR _at_sep _at_as_Rep /=.
           iFrame "CI". iFrame. iPureIntro. auto.
-        + iDestruct "State" as "(P & Owner & OF & Balance)".
-          iEval (rewrite /LockState.not_locked /LockState.token) in "NL".
-          iDestruct "NL" as "[Sets T]".
-          iDestruct (MutexTokens.acquire with "[$Balance $T]") as "[GT Balance]".
-          iMod (LockState.owner_update _ _ _ (Some thr) with "[$OA $OF]")
-            as "[OA OF]".
-          iMod ("Hclose" with "[L OA Sets Balance]") as "_".
+        + iDestruct "Resources" as "[P Owner]".
+          iMod (State.do_lock with "[$State $NL]") as "[State Locked]".
+          iMod ("Hclose" with "[L State]") as "_".
           { iNext. rewrite /mutex_inv. iExists true.
             iSplitL "L"; first by ework $usenamed=true with br_erefl.
-            iExists (Some thr). iFrame "OA".
-            iExists thr. iFrame. done. }
-          iModIntro. rewrite /IR _at_sep _at_as_Rep /LockState.locked /=.
+            iFrame. }
+          iModIntro. rewrite /IR _at_sep _at_as_Rep /=.
           iFrame "CI". iFrame. iPureIntro. auto.
     Qed.
     Hint Resolve do_exchange_C : sl_opacity.
@@ -287,10 +424,10 @@ Module custom_mutex.
       \consuming{g q P} p |-> IR g q P
       \consuming P
       \consuming p ,, _field "MyMutex::m_owner" |-> thread_idR 1$m None
-      \consuming LockState.locked g.(lock_state_gname) (Some thr) q
+      \consuming State.owner_token g thr q
       \proving{K (_ : IsExistential K)}
         std.atomic.do_store "int" (BASE (p ,, o_field σ "MyMutex::m_lock")) 0%Z K
-      \instantiate K := (p |-> IR g q P ** LockState.not_locked g.(lock_state_gname) thr q g.(cinv_gname))
+      \instantiate K := (p |-> IR g q P ** State.lock_permit g thr q)
       \end@{mpredI}.
     Next Obligation.
       intros. iIntros "[#M Hpre]" (?? ->).
@@ -298,33 +435,26 @@ Module custom_mutex.
       iDestruct "Hpre" as "(#Thr & IR & P & Owner & Locked)".
       iEval (rewrite /IR _at_sep _at_as_Rep) in "IR".
       iDestruct "IR" as "(S & #CI & CO)".
-      iEval (rewrite /LockState.locked) in "Locked".
-      iDestruct "Locked" as "[GT OF]".
       rewrite /std.atomic.do_store.
       iAcIntro. rewrite /commit_acc /=.
       iInv lock_namespace as "Inv" "Hclose".
       iDestruct "Inv" as "[Inv CO]".
       iEval (rewrite /mutex_inv) in "Inv".
-      iDestruct "Inv" as (b) "[>L Inv]".
-      iDestruct "Inv" as (oo) "[>OA State]".
+      iDestruct "Inv" as (b) "(>L & State & Resources)".
       iDestruct (fupd_mask_subseteq) as ">Y"; [ | iModIntro ]; first set_solver.
       iExists (if b then 1 else 0)%Z.
       iSplitL "L"; first by ework $usenamed=true with br_erefl.
       iNext. iIntros "L". iMod "Y" as "_".
       destruct b.
-      - iDestruct "State" as (owner) "(Sets & %Heq & Balance)".
-        iDestruct (observe_2 [| oo = Some thr |] with "OA OF") as %Howner.
-        have -> : owner = thr by congruence.
-        iDestruct (MutexTokens.release with "[$Balance $GT]") as "[T Balance]".
-        iMod ("Hclose" with "[L OA P Owner OF Balance]") as "_".
+      - iMod (State.do_unlock with "[$State $Locked]") as "[State NL]".
+        iMod ("Hclose" with "[L State P Owner]") as "_".
         { iNext. rewrite /mutex_inv. iExists false.
           iSplitL "L"; first by ework $usenamed=true with br_erefl.
-          iExists oo. iFrame. by rewrite Howner. }
+          iFrame. }
         iModIntro.
-        rewrite /IR _at_sep _at_as_Rep /LockState.not_locked /=.
+        rewrite /IR _at_sep _at_as_Rep /=.
         iFrame "CI". iFrame.
-      - iDestruct "State" as "(P0 & Owner0 & OF0 & Balance0)".
-        iDestruct (LockState.owner_tid_frag_exclusive with "OF0 OF") as %[].
+      - iDestruct (State.unlocked_owner_token with "[$State $Locked]") as %[].
     Qed.
     Hint Resolve do_store_C : sl_opacity.
 
@@ -350,8 +480,6 @@ Module custom_mutex.
     Qed.
     Hint Resolve do_load_C : sl_opacity.
 
-    Hint Opaque lockedR : sl_opacity.
-
     Lemma mymutex_do_lock_proof : verify[source] "MyMutex::do_lock()".
     Proof using MOD HAS_THREADS.
       verify_spec; go.
@@ -367,17 +495,14 @@ Module custom_mutex.
     Lemma mymutex_lock_alt_proof : verify[source] lock_spec_alt.
     Proof using MOD HAS_THREADS.
       verify_spec; ego.
-      rewrite lockedR.unlock.
-      ego.
-      Unshelve. all: first [exact (1$m)%cQp | exact tt].
+      Unshelve. all: exact (1$m)%cQp.
     Qed.
 
     Lemma mymutex_unlock_alt_proof : verify[source] unlock_spec_alt.
     Proof using MOD HAS_THREADS.
       verify_spec.
-      rewrite lockedR.unlock.
       repeat (go; ework).
-      Unshelve. all: first [exact (1$m)%cQp | exact tt].
+      Unshelve. all: exact (1$m)%cQp.
     Qed.
 
     Lemma mymutex_ctor_proof : verify[source] "MyMutex::MyMutex()".
@@ -387,21 +512,16 @@ Module custom_mutex.
       wname [P] "P".
       wname [_ |-> atomic.R _ _ _] "L".
       wname [_ |-> thread_idR _ _] "Owner".
-      iMod (MutexSets.alloc_pool (nroot .@@ "MyMutexPool")) as (gp) "#Pool".
-      iMod (MutexTokens.alloc) as (gt) "[T GT]".
-      iMod (own_alloc ((●E None ⋅ ◯E None) : LockState.owner_cmraR)) as (go) "O".
-      { apply excl_auth_valid. }
-      iDestruct (own_op with "O") as "[OA OF]".
-      pose (gs := LockState.MkGname (nroot .@@ "MyMutexPool") gp gt go).
       iMod (cinv_alloc_cofinite ∅ ⊤ lock_namespace) as (gi) "(_ & CO & Halloc)".
-      iMod ("Halloc" $! (mutex_inv this (MkGname gs gi) P)
-        with "[] [L P Owner OA OF GT]") as "#CI".
+      iMod (State.alloc γpool gi) as (gs) "(%Hpool & %Hinv & T & State)".
+      iMod ("Halloc" $! (mutex_inv this gs P)
+        with "[] [L P Owner State]") as "#CI".
       { iPureIntro. rewrite /mutex_inv. apply _. }
-      { iNext. rewrite /mutex_inv /=. iExists false. iFrame "L".
-        iExists None. rewrite /LockState.owner_tid_auth /LockState.owner_tid_frag /gs /=.
-        iFrame. rewrite /MutexTokens.token_full. iLeft. iExact "GT". }
-      iModIntro. iExists (MkGname gs gi).
-      rewrite /IR _at_sep _at_as_Rep /LockState.token /gs /=.
+      { iNext. rewrite /mutex_inv /=. iExists false. iFrame. }
+      iModIntro. iExists gs.
+      iSplit; first done.
+      subst gi.
+      rewrite /IR _at_sep _at_as_Rep /cinv_gname /=.
       iFrame "CI". iFrame.
     Qed.
 
@@ -412,31 +532,30 @@ Module custom_mutex.
       work.
       wname [cinv] "#CI".
       wname [cinv_own] "CO".
-      wname [LockState.token] "T".
+      wname [State.token] "T".
       iMod (cinv_cancel with "CI CO")
         as "Inv"; [done..|].
       go.
-      iDestruct "Inv" as (b) "(Lock & % & OA & State)".
-      destruct b eqn:Hb.
-      - iDestruct "State" as (th) "(Sets & %Eq & Balance)".
-        iEval (rewrite /LockState.token) in "T".
-        iDestruct (MutexTokens.token_not_full_full_token with "[$Balance $T]") as %[].
-      - iDestruct "State" as "(P & Owner & OF & Balance)".
+      iDestruct "Inv" as (b) "(Lock & State & Resources)".
+      destruct b.
+      - iDestruct (State.locked_full_token with "[$State $T]") as %[].
+      - iDestruct "Resources" as "[P Owner]".
+        iAssert emp with "[State T]" as "_".
+        { iApply (affine with "[State T]"); last iAccu. apply mpred_BiAffine. }
         ego $usenamed=true with br_erefl.
-        iApply (affine with "[OA OF Balance T]"); last iAccu. apply mpred_BiAffine.
     Qed.
 
     Lemma mymutex_lock_proof : verify[source] lock_spec.
     Proof using MOD HAS_THREADS.
       have -> : lock_spec ⊣⊢ lock_spec_alt.
-      { apply (Spec.lock_spec_entails_lock_spec_alt mutexR not_locked locked). done. }
+      { apply (Spec.lock_spec_entails_lock_spec_alt mutexR (fun g => g)). done. }
       exact mymutex_lock_alt_proof.
     Qed.
 
     Lemma mymutex_unlock_proof : verify[source] unlock_spec.
     Proof using MOD HAS_THREADS.
       have -> : unlock_spec ⊣⊢ unlock_spec_alt.
-      { apply (Spec.unlock_spec_entails_unlock_spec_alt mutexR not_locked_raw locked_raw). done. }
+      { apply (Spec.unlock_spec_entails_unlock_spec_alt mutexR (fun g => g)). done. }
       exact mymutex_unlock_alt_proof.
     Qed.
 
